src/hmem/encoding/emulator.lean
@@ -1,0 +1,45 @@
+import hmem.stack
+import hmem.encoding.basic
+import hmem.split_cost
+import hmem.trace
+import complexity.basic
+
+variables {μ: Type*} [decidable_eq μ] [has_zero μ] [has_one μ] [ne_zero (1:μ)]
+
+namespace hmem
+namespace encoding
+
+
+instance: complexity.has_encoding (runtime_model μ) (memory μ) :=
+⟨ ⟨ id, λ _ _, by refl  ⟩ ⟩
+
+noncomputable instance {α: Type*} [complexity.has_encoding (runtime_model μ) α]:
+  complexity.has_encoding (runtime_model μ) (μ → α) :=
+begin
+  fconstructor,
+  fconstructor,
+  exact λ f, quotient.mk (hidden.memory.node (0:μ) (λ u, quotient.out (encode (f u)))),
+  intros x y,
+  split,
+  intro p,
+  funext u,
+  have h := congr_fun (congr_arg memory.getm p) u,
+  rw [memory.getm_mk, memory.getm_mk] at h,
+  unfold hidden.getm at h,
+  rw [quotient.out_eq, quotient.out_eq] at h,
+  apply encode_inj h,
+  intro h,
+  rw [h],
+  exact rfl,
+end
+
+-- def encode_instruction: instruction μ → memory μ
+-- | vop {n: ℕ} (op: vector α n → α) (dst: source α) (src: vector (source α) n): instruction
+-- | mop (op: hmem.instruction.memory_operation) (dst src: source α): instruction
+-- | clear (dst: source α): instruction
+-- | ite {n: ℕ} (cond: vector α n → Prop) [Π {v}, decidable (cond v)] (src: vector (source α) n) (branch: list instruction): instruction
+-- | call (func: list instruction) (dst src: source α): instruction
+-- | recurse (dst src: source α): instruction
+
+end encoding
+end hmem
